minor: update `blake_air::air`

CoqOfRust/plonky3/blake3_air/links/air.v
@@ -1,41 +1,185 @@
 Require Import CoqOfRust.CoqOfRust.
 Require Import CoqOfRust.links.M.
 Require Import plonky3.blake3_air.air.
+Require Import plonky3.field.links.field.
+Require Import plonky3.blake3_air.links.columns.
+Require Import plonky3.air.links.air.
+Require Import plonky3.matrix.links.dense.
+
+(* 
+TODO:
+- Move all files under `src` to their parent files for consistency
+- In future, refer to `gas` to deal with different impls
+- In future, for all dependencies, fix their type path to actual path that starts with `p_3`
+- Check if AirBuilder needs `AB_types`
+*)
 
 (* pub struct Blake3Air {} *)
 Module Blake3Air.
-  Inductive t : Set :=
-  | Make.
+  Record t : Set := {}.
+
+  Parameter to_value : t -> Value.t.
 
   Global Instance IsLink : Link t := {
-    Φ := Ty.path "plonky3::blake3-air::Blake3Air";
-    φ _ := Value.StructRecord "p3_blake3_air::air::Blake3Air" [] [] [];
+  (* TODO: fix path here *)
+    Φ := Ty.path "plonky3::blake3_air::air::Blake3Air";
+    φ := to_value;
   }.
 
-  Definition of_ty : OfTy.t (Ty.path "plonky3::blake3-air::Blake3Air").
+  Definition of_ty : OfTy.t (Ty.path "plonky3::blake3_air::air::Blake3Air").
   Proof. eapply OfTy.Make with (A := t); reflexivity. Defined.
-  Smpl Add apply of_ty : of_ty.
+  Smpl Add apply of_ty : of_ty. 
 End Blake3Air.
 
 Module Impl_Blake3Air.
-(* TODO: figure out what is this `PrimeField64` *)
-(* 
-impl Blake3Air {
-    pub fn generate_trace_rows<F: PrimeField64>(
-        &self,
-        num_hashes: usize,
-        extra_capacity_bits: usize,
-    ) -> RowMajorMatrix<F> {
-*)
-
-(* 
-  Instance run_STOP :
+  Definition Self := Blake3Air.t.
+  (* 
+  impl Blake3Air {
+      pub fn generate_trace_rows<F: PrimeField64>(
+          &self,
+          num_hashes: usize,
+          extra_capacity_bits: usize,
+      ) -> RowMajorMatrix<F>
+  *)
+  Instance run_generate_trace_rows
+    {F : Set} `{Link F} 
+    {run_PrimeField64_for_F : PrimeField64.Run F}
+    (self : Ref.t Pointer.Kind.Ref Self) (num_hashes : Usize.t) (extra_capacity_bits : Usize.t) :
     Run.Trait
-      opcode.Impl_revm_bytecode_opcode_OpCode.value_STOP [] [] []
-      (Ref.t Pointer.Kind.Raw OpCode.t).
+      blake3_air.air.air.Impl_p3_blake3_air_air_Blake3Air.generate_trace_rows [] [ Φ F ] [ φ num_hashes; φ extra_capacity_bits ]
+      (RowMajorMatrix.t F).
   Proof.
     constructor.
     run_symbolic.
-  Defined.
-*)
+  Admitted.
+
+  (* 
+  fn quarter_round_function<AB: AirBuilder>(
+          &self,
+          builder: &mut AB,
+          trace: &QuarterRound<<AB as AirBuilder>::Var, <AB as AirBuilder>::Expr>,
+      )
+  *)
+  Instance run_quarter_round_function
+    {AB : Set} `{Link AB} 
+    {run_AirBuilder_for_AB : AirBuilder.Run AB}
+    (* TODO: check if AirBuilder needs `AB_types` *)
+    (self : Ref.t Pointer.Kind.Ref Self) 
+    (builder : Ref.t Pointer.Kind.MutRef AB) 
+    (* TODO: translate `trace: &QuarterRound<<AB as AirBuilder>::Var, <AB as AirBuilder>::Expr>` *)
+    (trace : Set)
+    :
+    Run.Trait
+      blake3_air.air.air.Impl_p3_blake3_air_air_Blake3Air.quarter_round_function [] [ Φ AB ] [ φ builder (* ; φ trace *) ]
+      unit.
+  Proof.
+    constructor.
+    run_symbolic.
+  Admitted.
+
+  (* 
+  const fn full_round_to_column_quarter_round<'a, T: Copy, U>(
+      &self,
+      input: &'a Blake3State<T>,
+      round_data: &'a FullRound<T>,
+      m_vector: &'a [[U; 2]; 16],
+      index: usize,
+  ) -> QuarterRound<'a, T, U>
+  *)
+  Instance run_full_round_to_column_quarter_round
+  (* NOTE: seems like there are some issues with T and U being defined here *)
+    {T U : Set} `{Link T}  `{Link U}
+    (self : Ref.t Pointer.Kind.Ref Self) 
+    (input : Ref.t Pointer.Kind.Ref (Blake3State.t T))
+    (round_data : Ref.t Pointer.Kind.Ref (FullRound.t T))
+    (m_vector : list (list U))
+    (index : Usize.t)
+    :
+    Run.Trait
+      blake3_air.air.air.Impl_p3_blake3_air_air_Blake3Air.full_round_to_column_quarter_round [] [ Φ T; Φ U ] 
+      [ (* φ input; φ round_data; φ m_vector; φ index *) ]
+      (QuarterRound.t T U).
+  Proof.
+    constructor.
+    run_symbolic.
+  Admitted.
+
+  (* 
+  const fn full_round_to_diagonal_quarter_round<'a, T: Copy, U>(
+      &self,
+      round_data: &'a FullRound<T>,
+      m_vector: &'a [[U; 2]; 16],
+      index: usize,
+  ) -> QuarterRound<'a, T, U> 
+  *)
+  Instance run_full_round_to_diagonal_quarter_round
+    {T U : Set} `{Link T}  `{Link U}
+    (self : Ref.t Pointer.Kind.Ref Self) 
+    (round_data : Ref.t Pointer.Kind.Ref (FullRound.t T))
+    (m_vector : list (list U))
+    (index : Usize.t)
+    :
+    Run.Trait
+      blake3_air.air.air.Impl_p3_blake3_air_air_Blake3Air.full_round_to_diagonal_quarter_round [] [ Φ T; Φ U ] 
+      [ (* φ input; φ round_data; φ m_vector; φ index *) ]
+      (QuarterRound.t T U).
+  Proof.
+    constructor.
+    run_symbolic.
+  Admitted.
+
+  (* 
+  fn verify_round<AB: AirBuilder>(
+      &self,
+      builder: &mut AB,
+      input: &Blake3State<AB::Var>,
+      round_data: &FullRound<AB::Var>,
+      m_vector: &[[AB::Expr; 2]; 16],
+  )
+  *)
+  Instance run_verify_round
+    {AB : Set} `{Link AB} 
+    {run_AirBuilder_for_AB : AirBuilder.Run AB}
+    (self : Ref.t Pointer.Kind.Ref Self) 
+    (builder : Ref.t Pointer.Kind.MutRef AB) 
+    (* TODO: translate correctly the following variables *)
+    (* (input : Ref.t Pointer.Kind.Ref Blake3State.t (AB.Var)) *)
+    (* (round_data : Ref.t Pointer.Kind.Ref FullRound (AB.Var)) *)
+    (* (m_vector : list (list Set)) *)
+    :
+    Run.Trait
+      blake3_air.air.air.Impl_p3_blake3_air_air_Blake3Air.verify_round [] [ Φ AB ] 
+        [ φ builder (* ; φ input; φ round_data; φ m_vector *) ]
+      unit.
+  Proof.
+    constructor.
+    run_symbolic.
+  Admitted.
 End Impl_Blake3Air.
+
+(* 
+impl<F> BaseAir<F> for Blake3Air {
+    fn width(&self) -> usize {
+        NUM_BLAKE3_COLS
+    }
+}
+*)
+Module Impl_BaseAir_for_Blake3Air.
+  Definition Self : Set :=
+    Blake3Air.t.
+
+  (* Instance run : BaseAir.Run Self. *)
+  (* Admitted. *)
+End Impl_BaseAir_for_Blake3Air.
+
+(* 
+impl<AB: AirBuilder> Air<AB> for Blake3Air {
+    fn eval(&self, builder: &mut AB)
+*)
+Module Impl_Air_for_Blake3Air.
+  Definition Self : Set :=
+    Blake3Air.t.
+
+  (* Instance run : Air.Run Self. *)
+  (* Admitted. *)
+End Impl_Air_for_Blake3Air.
